rt ainvs: DetSched projections as primrec
This commit converts existing AInvs DetSched projections (tcb_of, sc_of
and ep_of) to be defined as primrec. It also adds ntfn_of and reply_of.
Defining them as primrec seems to work well in terms of simplification
and often results in simpler codes.

--

So far, tcb_of and sc_of in AInvs are case statements on kernel objects
defined as definitions, and they needed to be explicitly unfolded to
simplify to an option value.

Making them abbreviations is one way to automate the simplification, but
it has a drawback in that the case statement often has unfortunate
interaction with Map.empty, which is an abbreviation of its own, that
tends to produce unwantedly expanded case expressions in subgoals.

It is probably possible to automate the simplication of definitions
by writing a simplification rule for each kernel object case and add
all of such rules to the simp set, but defining these projections as
primrec seems to work just as well, and it also often results in
shorter proofs as we can skip case distinctions which would be needed
otherwise.

Signed-off-by: Miki Tanaka <miki.tanaka@data61.csiro.au>

proof/invariant-abstract/DetSchedInvs_AI.thy
@@ -581,26 +581,30 @@ end
 
 \<comment> \<open>Project threads from the kernel heap\<close>
 
-definition tcb_of :: "kernel_object \<rightharpoonup> tcb" where
-  "tcb_of ko \<equiv> case ko of TCB tcb \<Rightarrow> Some tcb | _ \<Rightarrow> None"
-
-lemma tcb_of_simps:
+primrec tcb_of :: "Structures_A.kernel_object \<rightharpoonup> tcb" where
   "tcb_of (TCB tcb) = Some tcb"
-  "tcb_of (SchedContext sc n) = None"
-  "tcb_of (CNode n cnode) = None"
-  "tcb_of (Endpoint ep) = None"
-  "tcb_of (Notification ntfn) = None"
-  "tcb_of (Reply reply) = None"
-  "tcb_of (ArchObj aobj) = None"
-  by (auto simp: tcb_of_def)
+| "tcb_of (Endpoint _) = None"
+| "tcb_of (Notification _) = None"
+| "tcb_of (CNode _ _) = None"
+| "tcb_of (Reply _) = None"
+| "tcb_of (SchedContext _ _) = None"
+| "tcb_of (ArchObj _) = None"
+
+lemma tcb_of_SomeD[dest!]:
+  "tcb_of ko = Some obj \<Longrightarrow> ko = TCB obj"
+  by (cases ko; simp)
+
+lemma tcb_of_NoneD[simp]:
+  "tcb_of ko = None \<Longrightarrow> \<not> (\<exists>tcb. ko = TCB tcb)"
+  by (cases ko; simp)
 
 lemma tcb_of_Some:
   "tcb_of ko = Some tcb \<longleftrightarrow> ko = TCB tcb"
-  by (simp add: tcb_of_def split: kernel_object.splits)
+  by (cases ko; simp)
 
 lemma tcb_of_None:
   "tcb_of ko = None \<longleftrightarrow> (\<forall>tcb. ko \<noteq> TCB tcb)"
-  by (simp add: tcb_of_def split: kernel_object.splits)
+  by (cases ko; simp)
 
 definition tcbs_of_kh :: "('obj_ref \<rightharpoonup> kernel_object) \<Rightarrow> 'obj_ref \<rightharpoonup> tcb" where
   "tcbs_of_kh kh \<equiv> kh |> tcb_of"
@@ -720,26 +724,30 @@ lemma etcb_at'_pred_map:
 
 \<comment> \<open>Project scheduling contexts from the kernel heap\<close>
 
-definition sc_of :: "kernel_object \<rightharpoonup> sched_context" where
-  "sc_of ko \<equiv> case ko of SchedContext sc n \<Rightarrow> Some sc | _ \<Rightarrow> None"
-
-lemma sc_of_simps:
-  "sc_of (SchedContext sc n) = Some sc"
-  "sc_of (CNode n cnode) = None"
+primrec sc_of :: "Structures_A.kernel_object \<rightharpoonup> sched_context" where
   "sc_of (TCB tcb) = None"
-  "sc_of (Endpoint ep) = None"
-  "sc_of (Notification ntfn) = None"
-  "sc_of (Reply reply) = None"
-  "sc_of (ArchObj aobj) = None"
-  by (auto simp: sc_of_def)
+| "sc_of (Endpoint _) = None"
+| "sc_of (Notification _) = None"
+| "sc_of (CNode _ _) = None"
+| "sc_of (Reply _) = None"
+| "sc_of (SchedContext sc _) = Some sc"
+| "sc_of (ArchObj _) = None"
+
+lemma sc_of_SomeD[dest!]:
+  "sc_of ko = Some obj \<Longrightarrow> \<exists>n. ko = SchedContext obj n"
+  by (cases ko; simp)
+
+lemma sc_of_NoneD[simp]:
+  "sc_of ko = None \<Longrightarrow> \<not> (\<exists>sc n. ko = SchedContext sc n)"
+  by (cases ko; simp)
 
 lemma sc_of_Some:
   "sc_of ko = Some sc \<longleftrightarrow> (\<exists>n. ko = SchedContext sc n)"
-  by (simp add: sc_of_def split: kernel_object.splits)
+ by (cases ko; simp)
 
 lemma sc_of_None:
   "sc_of ko = None \<longleftrightarrow> (\<forall>sc n. ko \<noteq> SchedContext sc n)"
-  by (simp add: sc_of_def split: kernel_object.splits)
+ by (cases ko; simp)
 
 definition scs_of_kh :: "('obj_ref \<rightharpoonup> kernel_object) \<Rightarrow> 'obj_ref \<rightharpoonup> sched_context" where
   "scs_of_kh kh \<equiv> kh |> sc_of"
@@ -835,54 +843,47 @@ global_interpretation sc_replies:
 
 \<comment> \<open>Project endpoints from the kernel heap\<close>
 
-definition ep_of :: "kernel_object \<rightharpoonup> endpoint" where
-  "ep_of ko \<equiv> case ko of Endpoint endpoint \<Rightarrow> Some endpoint | _ \<Rightarrow> None"
-
-definition send_q_of :: "endpoint \<rightharpoonup> obj_ref list" where
-  "send_q_of endpoint \<equiv> case endpoint of SendEP q  \<Rightarrow> Some q | _ \<Rightarrow> None"
-
-definition recv_q_of :: "endpoint \<rightharpoonup> obj_ref list" where
-  "recv_q_of endpoint \<equiv> case endpoint of RecvEP q  \<Rightarrow> Some q | _ \<Rightarrow> None"
-
-lemma ep_of_simps:
-  "ep_of (SchedContext sc n) = None"
-  "ep_of (CNode n cnode) = None"
+primrec ep_of :: "Structures_A.kernel_object \<rightharpoonup> endpoint" where
   "ep_of (TCB tcb) = None"
-  "ep_of (Endpoint endpoint) = Some endpoint"
-  "ep_of (Notification ntfn) = None"
-  "ep_of (Reply reply) = None"
-  "ep_of (ArchObj aobj) = None"
-  "send_q_of IdleEP = None"
+| "ep_of (Endpoint ep) = Some ep"
+| "ep_of (Notification _) = None"
+| "ep_of (CNode _ _) = None"
+| "ep_of (Reply _) = None"
+| "ep_of (SchedContext _ _) = None"
+| "ep_of (ArchObj _) = None"
+
+lemma ep_of_SomeD[dest!]:
+  "ep_of ko = Some obj \<Longrightarrow> ko = Endpoint obj"
+  by (cases ko; simp)
+
+lemma ep_of_NoneD[simp]:
+  "ep_of ko = None \<Longrightarrow> \<not> (\<exists>ep. ko = Endpoint ep)"
+  by (cases ko; simp)
+
+primrec send_q_of :: "endpoint \<rightharpoonup> obj_ref list" where
   "send_q_of (SendEP q) = Some q"
-  "send_q_of (RecvEP q) = None"
-  "recv_q_of IdleEP = None"
-  "recv_q_of (SendEP q) = None"
+| "send_q_of (RecvEP _)  = None"
+| "send_q_of IdleEP = None"
+
+primrec recv_q_of :: "endpoint \<rightharpoonup> obj_ref list" where
   "recv_q_of (RecvEP q) = Some q"
-  by (auto simp: ep_of_def send_q_of_def recv_q_of_def)
+| "recv_q_of (SendEP _)  = None"
+| "recv_q_of IdleEP = None"
 
 lemma ep_of_Some:
   "ep_of ko = Some ep \<longleftrightarrow> ko = Endpoint ep"
-  by (simp add: ep_of_def split: kernel_object.splits)
+  by (cases ko; simp)
 
 lemma ep_of_None:
   "ep_of ko = None \<longleftrightarrow> (\<forall>ep. ko \<noteq> Endpoint ep)"
-  by (simp add: ep_of_def split: kernel_object.splits)
+  by (cases ko; simp)
 
-lemma send_q_of_Some:
-  "send_q_of ep = Some q \<longleftrightarrow> ep = SendEP q"
-  by (simp add: send_q_of_def split: endpoint.splits)
-
-lemma send_q_of_None:
-  "send_q_of ep = None \<longleftrightarrow> (\<forall>q. ep \<noteq> SendEP q)"
-  by (simp add: send_q_of_def split: endpoint.splits)
-
-lemma recv_q_of_Some:
-  "recv_q_of ep = Some q \<longleftrightarrow> ep = RecvEP q"
-  by (simp add: recv_q_of_def split: endpoint.splits)
-
-lemma recv_q_of_None:
-  "recv_q_of ep = None \<longleftrightarrow> (\<forall>q. ep \<noteq> RecvEP q)"
-  by (simp add: recv_q_of_def split: endpoint.splits)
+lemma shows
+  send_q_of_Some: "send_q_of ep = Some q \<longleftrightarrow> ep = SendEP q" and
+  send_q_of_None: "send_q_of ep = None \<longleftrightarrow> (\<forall>q. ep \<noteq> SendEP q)" and
+  recv_q_of_Some: "recv_q_of ep = Some q \<longleftrightarrow> ep = RecvEP q" and
+  recv_q_of_None: "recv_q_of ep = None \<longleftrightarrow> (\<forall>q. ep \<noteq> RecvEP q)"
+  by (cases ep; simp)+
 
 definition eps_of_kh :: "('obj_ref \<rightharpoonup> kernel_object) \<Rightarrow> 'obj_ref \<rightharpoonup> endpoint" where
   "eps_of_kh kh \<equiv> kh |> ep_of"
@@ -916,6 +917,54 @@ global_interpretation ep_recv_qs:
   opt_map_opt_map_cons_def_locale _ ep_of eps_of_kh Endpoint recv_q_of RecvEP ep_recv_qs_of_eps
   using ep_recv_qs_of_eps_def recv_q_of_None recv_q_of_Some by unfold_locales
 
+\<comment> \<open>Notifications\<close>
+
+\<comment> \<open>Project notifications from the kernel heap\<close>
+
+primrec ntfn_of :: "Structures_A.kernel_object \<rightharpoonup> notification" where
+  "ntfn_of (TCB tcb) = None"
+| "ntfn_of (Endpoint ep) = None"
+| "ntfn_of (Notification ntfn) = Some ntfn"
+| "ntfn_of (CNode _ _) = None"
+| "ntfn_of (Reply _) = None"
+| "ntfn_of (SchedContext _ _) = None"
+| "ntfn_of (ArchObj _) = None"
+
+lemma ntfn_of_SomeD[dest!]:
+  "ntfn_of ko = Some obj \<Longrightarrow> ko = Notification obj"
+  by (cases ko; simp)
+
+lemma ntfn_of_NoneD[simp]:
+  "ntfn_of ko = None \<Longrightarrow> \<not> (\<exists>ep. ko = Notification ep)"
+  by (cases ko; simp)
+
+abbreviation ntfns_of :: "'z state \<Rightarrow> obj_ref \<rightharpoonup> Structures_A.notification" where
+  "ntfns_of \<equiv> (\<lambda>s. kheap s |> ntfn_of)"
+
+\<comment> \<open>Replies\<close>
+
+\<comment> \<open>Project replies from the kernel heap\<close>
+
+primrec reply_of :: "Structures_A.kernel_object \<rightharpoonup> reply" where
+  "reply_of (TCB tcb) = None"
+| "reply_of (Endpoint ep) = None"
+| "reply_of (Notification _) = None"
+| "reply_of (CNode _ _) = None"
+| "reply_of (Reply reply) = Some reply"
+| "reply_of (SchedContext _ _) = None"
+| "reply_of (ArchObj _) = None"
+
+lemma reply_of_SomeD[dest!]:
+  "reply_of ko = Some obj \<Longrightarrow> ko = Reply obj"
+  by (cases ko; simp)
+
+lemma reply_of_NoneD[simp]:
+  "reply_of ko = None \<Longrightarrow> \<not> (\<exists>reply. ko = Reply reply)"
+  by (cases ko; simp)
+
+abbreviation replies_of :: "'z state \<Rightarrow> obj_ref \<rightharpoonup> Structures_A.reply" where
+  "replies_of \<equiv> (\<lambda>s. kheap s |> reply_of)"
+
 \<comment> \<open>Heap simplification rules\<close>
 
 lemmas vs_pred_map_simps =
@@ -948,9 +997,6 @@ lemmas vs_pred_map_simps =
   pred_map_def[where m="kheap s" for s :: "'z state"]
 
 lemmas vs_heap_simps =
-  tcb_of_simps
-  sc_of_simps
-  ep_of_simps
   tcb_heap.simps
   tcb_sts.simps
   tcb_scps.simps
